AND_AND_2 optimization (not finished)

ver2/optimizations/and_and2.v
@@ -57,13 +57,15 @@ Require Import List.
 Import ListNotations.
 
 
-Module Opt_and_and1.
+Module Opt_and_and2.
 
+(* sv1 sv2 maxidx1 sb1 maxid2 sb2 instk_height ops -> bool *)
+Definition sstack_val_cmp_t := sstack_val -> sstack_val -> nat -> sbindings -> nat -> sbindings -> nat -> stack_op_instr_map -> bool.
 
-(* AND(X,AND(X,Y)) = AND(X,Y)
-   AND(X,AND(Y,X)) = AND(X,Y)
+(* AND(AND(X,Y), X) = AND(X,Y)
+   AND(AND(X,Y), Y) = AND(X,Y)
  *)
-Definition optimize_and_and1_sbinding : opt_smap_value_type := 
+Definition optimize_and_and2_sbinding : opt_smap_value_type := 
 fun (val: smap_value) =>
 fun (fcmp: sstack_val_cmp_t) =>
 fun (sb: sbindings) =>
@@ -72,12 +74,12 @@ fun (instk_height: nat) =>
 fun (ops: stack_op_instr_map) => 
 match val with
 | SymOp AND [arg1;arg2] => 
-  match follow_in_smap arg2 maxid sb with
-  | Some (FollowSmapVal (SymOp AND [arg21;arg22]) idx' sb') => 
-      if fcmp arg1 arg21 maxid sb idx' sb' instk_height ops then 
-        (SymOp AND [arg1;arg22], true)
-      else if fcmp arg1 arg22 maxid sb idx' sb' instk_height ops then 
-        (SymOp AND [arg1;arg21], true)
+  match follow_in_smap arg1 maxid sb with
+  | Some (FollowSmapVal (SymOp AND [arg11;arg12]) idx' sb') => 
+      if fcmp arg11 arg2 idx' sb' maxid sb instk_height ops then 
+        (SymOp AND [arg11;arg12], true)
+      else if fcmp arg12 arg2 idx' sb' maxid sb instk_height ops then 
+        (SymOp AND [arg2;arg11], true)
       else 
         (val, false)
   | _ => (val, false)
@@ -98,20 +100,20 @@ induction x as [|b n x' IH].
 Qed.
 
 
-Lemma wand_wand1_1: forall (x y: EVMWord),
-wand x (wand x y) = wand x y.
+Lemma wand_wand2_1: forall (x y: EVMWord),
+wand (wand x y) x = wand x y.
 Proof.
 intros x y.
+rewrite -> wand_comm.
 rewrite -> wand_assoc.
 rewrite -> wand_x_x.
 reflexivity.
 Qed.
 
-Lemma wand_wand1_2: forall (x y: EVMWord),
-wand x (wand y x) = wand x y.
+Lemma wand_wand2_2: forall (x y: EVMWord),
+wand (wand x y) y = wand x y.
 Proof.
 intros x y.
-rewrite -> wand_comm.
 rewrite <- wand_assoc.
 rewrite -> wand_x_x.
 rewrite -> wand_comm.
@@ -119,28 +121,28 @@ reflexivity.
 Qed.
 
 
-Lemma optimize_and_and1_sbinding_smapv_valid:
-opt_smapv_valid_snd optimize_and_and1_sbinding.
+Lemma optimize_and_and2_sbinding_smapv_valid:
+opt_smapv_valid_snd optimize_and_and2_sbinding.
 Proof.
 unfold opt_smapv_valid_snd.
 intros instk_height n ops fcmp sb val val' flag.
 intros Hvalid_smapv_val Hvalid Hoptm_sbinding.
-unfold optimize_and_and1_sbinding in Hoptm_sbinding.
+unfold optimize_and_and2_sbinding in Hoptm_sbinding.
 destruct (val) as [basicv|pushtagv|label args|offset smem|key sstrg|
   offset size smem] eqn: eq_val; 
   try inject_rw Hoptm_sbinding eq_val'.
 destruct label eqn: eq_label; try try inject_rw Hoptm_sbinding eq_val'.
 destruct args as [|arg1 r1]; try inject_rw Hoptm_sbinding eq_val'.
 destruct r1 as [|arg2 r2]; try inject_rw Hoptm_sbinding eq_val'.
-destruct r2 as [|arg3 r3]; try inject_rw Hoptm_sbinding eq_val'.
-destruct (follow_in_smap arg2 n sb) as [fsmv_arg2|] eqn: eq_follow_arg2;
+destruct r2; try inject_rw Hoptm_sbinding eq_val'.
+destruct (follow_in_smap arg1 n sb) as [fsmv_arg1|] eqn: eq_follow_arg1;
   try inject_rw Hoptm_sbinding eq_val'.
-destruct fsmv_arg2 as [smv_arg2 idx' sb'] eqn: eq_fsmv_arg2.
-destruct smv_arg2 as [x1|x2|label2 args2|x4|x5|x6] eqn: eq_smv;
+destruct fsmv_arg1 as [smv_arg1 idx' sb'] eqn: eq_fsmv_arg1.
+destruct smv_arg1 as [x1|x2|label2 args2|x4|x5|x6] eqn: eq_smv;
   try inject_rw Hoptm_sbinding eq_val'.
-destruct label2 eqn: eq_label2; try inject_rw Hoptm_sbinding eq_val'.
-destruct args2 as [|arg21 r21] eqn: eq_args2; try inject_rw Hoptm_sbinding eq_val'.
-destruct r21 as [|arg22 r22] eqn: eq_r21; try inject_rw Hoptm_sbinding eq_val'.
+destruct label2; try inject_rw Hoptm_sbinding eq_val'.
+destruct args2 as [|arg11 r12]; try inject_rw Hoptm_sbinding eq_val'.
+destruct r12 as [|arg12 r22]; try inject_rw Hoptm_sbinding eq_val'.
 destruct r22; try inject_rw Hoptm_sbinding eq_val'.
 
 assert (Hvalid_smapv_val_copy := Hvalid_smapv_val).
@@ -151,28 +153,29 @@ destruct Hvalid_smapv_val as [Hlen_nargs Hvalid_arg1_arg2].
 simpl in Hvalid_arg1_arg2.
 destruct Hvalid_arg1_arg2 as [Hvalid_arg1 [Hvalid_arg2]].
 
-pose proof (valid_follow_in_smap sb arg2 instk_height n ops
-      (SymOp AND [arg21; arg22]) idx' sb' Hvalid_arg2 Hvalid
-      eq_follow_arg2) as Hvalid2.
+pose proof (valid_follow_in_smap sb arg1 instk_height n ops
+      (SymOp AND [arg11; arg12]) idx' sb' Hvalid_arg1 Hvalid
+      eq_follow_arg1) as Hvalid2.
 destruct Hvalid2 as [Hvalid_smap [Hvalid_sb' Himpl]].
 simpl in Hvalid_smap. unfold valid_stack_op_instr in Hvalid_smap.
 rewrite -> eq_ops_and in Hvalid_smap.
-destruct Hvalid_smap as [Hlen_nargs' Hvalid_arg21_arg22].
-simpl in Hvalid_arg21_arg22.
-destruct Hvalid_arg21_arg22 as [Hvalid_arg21 [Hvalid_arg22 _]].
-pose proof (not_basic_value_smv_symop AND [arg21; arg22]) as eq_not_basic.
+destruct Hvalid_smap as [Hlen_nargs' Hvalid_arg11_arg12].
+simpl in Hvalid_arg11_arg12.
+destruct Hvalid_arg11_arg12 as [Hvalid_arg11 [Hvalid_arg12 _]].
+pose proof (not_basic_value_smv_symop AND [arg11; arg12]) as eq_not_basic.
 apply Himpl in eq_not_basic as n_gt_idx'.
 
-destruct (fcmp arg1 arg21 n sb idx' sb' instk_height ops) 
-  eqn: fcmp_arg1_arg21.
+destruct (fcmp arg11 arg2 idx' sb' n sb instk_height ops) 
+  eqn: fcmp_arg1_arg11.
 - injection Hoptm_sbinding as eq_val' _.
   rewrite <- eq_val'. 
   simpl. unfold valid_stack_op_instr. 
   rewrite -> eq_ops_and. split; try assumption. 
   simpl. split; try intuition.
   apply valid_sstack_value_gt with (n:=idx'); try assumption.
+  apply valid_sstack_value_gt with (n:=idx'); try assumption.
    
-- destruct (fcmp arg1 arg22 n sb idx' sb' instk_height ops) 
+- destruct (fcmp arg12 arg2 idx' sb' n sb instk_height ops) 
   eqn: fcmp_arg1_arg22; try inject_rw Hoptm_sbinding eq_val'.
   injection Hoptm_sbinding as eq_val' _.
   rewrite <- eq_val'. 
@@ -195,22 +198,23 @@ intros T x y.
 reflexivity.
 Qed.
 
+Search eval_sstack_val'.
 
 Lemma optimize_and_and1_sbinding_snd:
-opt_sbinding_snd optimize_and_and1_sbinding.
+opt_sbinding_snd optimize_and_and2_sbinding.
 Proof.
 unfold opt_sbinding_snd.
 intros val val' fcmp sb maxidx instk_height idx flag Hsafe_sstack_val_cmp
   Hvalid Hoptm_sbinding.
 split.
 - (* valid_sbindings *)
-  apply valid_bindings_snd_opt with (val:=val)(opt:=optimize_and_and1_sbinding)
+  apply valid_bindings_snd_opt with (val:=val)(opt:=optimize_and_and2_sbinding)
     (fcmp:=fcmp)(flag:=flag); try assumption.
-  apply optimize_and_and1_sbinding_smapv_valid. 
+  apply optimize_and_and2_sbinding_smapv_valid. 
 
 - (* evaluation is preserved *) 
   intros stk mem strg ctx v Hlen Heval_orig.
-  unfold optimize_and_and1_sbinding in Hoptm_sbinding.
+  unfold optimize_and_and2_sbinding in Hoptm_sbinding.
   destruct val as [vv|vv|label args|offset smem|key sstrg|offset seze smem]
     eqn: eq_val; try inject_rw Hoptm_sbinding eq_val'.
   (* SymOp label args *)
@@ -218,37 +222,40 @@ split.
   destruct args as [|arg1 r1] eqn: eq_args; 
     try inject_rw Hoptm_sbinding eq_val'.
   destruct r1 as [|arg2 r2]; try inject_rw Hoptm_sbinding eq_val'.
-  destruct r2 as [|arg3 r3]; try inject_rw Hoptm_sbinding eq_val'.
-  destruct (follow_in_smap arg2 idx sb) as [fsmv|] eqn: eq_follow_arg2;
+  destruct r2; try inject_rw Hoptm_sbinding eq_val'.
+  destruct (follow_in_smap arg1 idx sb) as [fsmv|] eqn: eq_follow_arg1;
     try inject_rw Hoptm_sbinding eq_val'.
   destruct fsmv as [smv idx' sb'] eqn: eq_fsmv.
   destruct smv as [_1|_2|label2 args2|_4|_5|_6] eqn: eq_smv;
     try inject_rw Hoptm_sbinding eq_val'.
   destruct label2 eqn: eq_label2; try inject_rw Hoptm_sbinding eq_val'.
-  destruct args2 as [|arg21 r21]; try inject_rw Hoptm_sbinding eq_val'.
-  destruct r21 as [|arg22 r22]; try inject_rw Hoptm_sbinding eq_val'.
+  destruct args2 as [|arg11 r21]; try inject_rw Hoptm_sbinding eq_val'.
+  destruct r21 as [|arg12 r22]; try inject_rw Hoptm_sbinding eq_val'.
   destruct r22; try inject_rw Hoptm_sbinding eq_val'.
   
   assert (Heval_orig_copy := Heval_orig).
   unfold eval_sstack_val in Heval_orig. simpl in Heval_orig.
   rewrite -> PeanoNat.Nat.eqb_refl in Heval_orig.
   simpl in Heval_orig.
-  destruct (eval_sstack_val' maxidx arg1 stk mem strg ctx idx sb evm_stack_opm)
-    as [arg1v|] eqn: eval_arg1; try discriminate.
-  destruct maxidx as [| maxidx']; try discriminate.
-  simpl in Heval_orig.
-  rewrite -> eq_follow_arg2 in Heval_orig.
-  simpl in Heval_orig.
-  destruct (eval_sstack_val' maxidx' arg21 stk mem strg ctx idx' sb' 
-    evm_stack_opm) as [arg21v|] eqn: eval_arg21; try discriminate.
-  destruct (eval_sstack_val' maxidx' arg22 stk mem strg ctx idx' sb' 
-    evm_stack_opm) as [arg22v|] eqn: eval_arg22; try discriminate.
+  destruct maxidx as [| maxidx'] eqn: eq_maxidx; try discriminate.
+  rewrite -> eval_sstack_val'_one_step in Heval_orig at 1.
+  rewrite -> eq_follow_arg1 in Heval_orig.
+  rewrite -> evm_stack_opm_AND in Heval_orig.
+  rewrite -> lenght2 in Heval_orig.
+  unfold map_option in Heval_orig.
+  destruct (eval_sstack_val' maxidx' arg11 stk mem strg ctx idx' sb' 
+    evm_stack_opm) as [arg11v|] eqn: eval_arg11; try discriminate.
+  destruct (eval_sstack_val' maxidx' arg12 stk mem strg ctx idx' sb' 
+    evm_stack_opm) as [arg12v|] eqn: eval_arg12; try discriminate.
+  destruct (eval_sstack_val' (S maxidx') arg2 stk mem strg ctx idx sb evm_stack_opm)
+    as [arg2v|] eqn: eval_arg2; try discriminate.
+    
+  injection Heval_orig as eq_v.
+  rewrite <- eq_v.
   
-  destruct (fcmp arg1 arg21 idx sb idx' sb' instk_height evm_stack_opm) 
-    eqn: eq_fcmp_arg1_arg21. 
-  + rewrite <- Heval_orig.
-    simpl.
-    injection Hoptm_sbinding as eq_val' _.
+  destruct (fcmp arg11 arg2 idx' sb' idx sb instk_height evm_stack_opm) 
+    eqn: eq_fcmp_arg11_arg2. 
+  + injection Hoptm_sbinding as eq_val' _.
     rewrite <- eq_val'.
     unfold eval_sstack_val.
     rewrite -> eval_sstack_val'_one_step. 
@@ -256,39 +263,85 @@ split.
     rewrite -> evm_stack_opm_AND. 
     rewrite -> lenght2.
     unfold map_option.
-    rewrite -> eval_arg1.
-    rewrite -> eval'_maxidx_indep_eq with (m:=idx) in eval_arg22.
-    apply eval_sstack_val'_preserved_when_depth_extended in eval_arg22.
-    pose proof (follow_suffix sb arg2 idx (SymOp AND [arg21; arg22]) idx' sb'
-      eq_follow_arg2) as Hprefix_sb.
+    
+    pose proof (follow_suffix sb arg1 idx (SymOp AND [arg11; arg12]) idx' sb'
+      eq_follow_arg1) as Hprefix_sb.
     destruct Hprefix_sb as [prefix Hprefix_sb].
     simpl in Hvalid.
-    destruct Hvalid as [eq_idx [Hvalid_stack_op Hvalid_sb]].    
-    pose proof (eval_sstack_val'_extend_sb instk_height (S maxidx') stk
-      mem strg ctx idx sb sb' evm_stack_opm prefix Hvalid_sb Hprefix_sb
-      arg22 arg22v eval_arg22) as Heval_arg22_sb.
-    rewrite -> Heval_arg22_sb. simpl.
-    
+    destruct Hvalid as [eq_idx [Hvalid_stack_op Hvalid_sb]].
     unfold valid_stack_op_instr in Hvalid_stack_op. simpl in Hvalid_stack_op.
     destruct Hvalid_stack_op as [_ [Hvalid_arg1 [Hvalid_arg2 _]]].
-    pose proof (valid_follow_in_smap sb arg2 instk_height idx evm_stack_opm
-      (SymOp AND [arg21; arg22]) idx' sb' Hvalid_arg2 Hvalid_sb
-      eq_follow_arg2) as Hvalid2.
+    
+    pose proof (valid_follow_in_smap sb arg1 instk_height idx evm_stack_opm
+      (SymOp AND [arg11; arg12]) idx' sb' Hvalid_arg1 Hvalid_sb
+      eq_follow_arg1) as Hvalid2.
     destruct Hvalid2 as [Hvalid_smapv_and [Hvalid_sb' Himpl]].
+    pose proof (not_basic_value_smv_symop AND [arg11;arg12]) as not_basic_and.
+    apply Himpl in not_basic_and.
+    
+    rewrite -> eval'_maxidx_indep_eq with (m:=idx) in eval_arg11.
+    rewrite -> eval'_maxidx_indep_eq with (m:=idx) in eval_arg12.
+    apply eval_sstack_val'_preserved_when_depth_extended in eval_arg11.
+    apply eval_sstack_val'_preserved_when_depth_extended in eval_arg12.
+    pose proof (eval_sstack_val'_extend_sb instk_height (S maxidx') stk
+      mem strg ctx idx sb sb' evm_stack_opm prefix Hvalid_sb Hprefix_sb
+      arg11 arg11v eval_arg11) as Heval_arg11_sb.
+    pose proof (eval_sstack_val'_extend_sb instk_height (S maxidx') stk
+      mem strg ctx idx sb sb' evm_stack_opm prefix Hvalid_sb Hprefix_sb
+      arg12 arg12v eval_arg12) as Heval_arg12_sb.
+    rewrite -> Heval_arg11_sb.
+    rewrite -> Heval_arg12_sb. simpl.
+    
+    (* arg11v must be equal to arg2v *)
+    (* TODO *)
+    symmetry in Hlen.
+    pose proof (Hsafe_sstack_val_cmp arg11 arg2 idx' sb' idx sb instk_height 
+      evm_stack_opm). Hvalid_arg11 Hvalid_arg2 Hvalid_sb' Hvalid_sb
+      eq_fcmp_arg11_arg2 stk mem strg ctx Hlen) as Hcmp_eval.
+    destruct Hcmp_eval as [vv [eval_arg11_vv eval_arg2_vv]].
+    
+(*    
+    apply eval_sstack_val'_preserved_when_depth_extended in eval_arg11.
+    rewrite -> eval_arg11.
+    rewrite -> eval'_maxidx_indep_eq with (m:=idx) in eval_arg12.
+    apply eval_sstack_val'_preserved_when_depth_extended in eval_arg12.
+    pose proof (follow_suffix sb arg1 idx (SymOp AND [arg11; arg12]) idx' sb'
+      eq_follow_arg1) as Hprefix_sb.
+    destruct Hprefix_sb as [prefix Hprefix_sb].
+    simpl in Hvalid.
+    destruct Hvalid as [eq_idx [Hvalid_stack_op Hvalid_sb]].
+    unfold valid_stack_op_instr in Hvalid_stack_op. simpl in Hvalid_stack_op.
+    destruct Hvalid_stack_op as [_ [Hvalid_arg1 [Hvalid_arg2 _]]].
+    
+    pose proof (valid_follow_in_smap sb arg1 instk_height idx evm_stack_opm
+      (SymOp AND [arg11; arg12]) idx' sb' Hvalid_arg1 Hvalid_sb
+      eq_follow_arg1) as Hvalid2.
+    destruct Hvalid2 as [Hvalid_smapv_and [Hvalid_sb' Himpl]].
+    
+    pose proof (eval_sstack_val'_extend_sb instk_height (S maxidx') stk
+      mem strg ctx idx sb sb' evm_stack_opm prefix Hvalid_sb Hprefix_sb
+      arg12 arg12v eval_arg12) as Heval_arg12_sb.
+    rewrite -> Heval_arg12_sb. simpl.
+    
+    (* arg11v must be equal to arg2v *)
+    (*TODO continue *)
     simpl in Hvalid_smapv_and. unfold valid_stack_op_instr in Hvalid_smapv_and.
     simpl in Hvalid_smapv_and.
-    destruct Hvalid_smapv_and as [_ [valid_arg21 [valid_arg22 _]]].
+    destruct Hvalid_smapv_and as [_ [valid_arg11 [valid_arg12 _]]].
+    
+    pose proof (not_basic_value_smv_symop AND [arg11;arg12]) as not_basic_and.
+    apply Himpl in not_basic_and as idx_gt_idx'.
      
     symmetry in Hlen.
-    pose proof (Hsafe_sstack_val_cmp arg1 arg21 idx sb idx' sb' instk_height 
-      evm_stack_opm Hvalid_arg1 valid_arg21 Hvalid_sb Hvalid_sb'
-      eq_fcmp_arg1_arg21 stk mem strg ctx Hlen) as Hcmp_eval.
-    destruct Hcmp_eval as [vv [eval_arg1_vv eval_arg21_vv]].
+    pose proof (Hsafe_sstack_val_cmp arg11 arg2 idx' sb' idx sb instk_height 
+      evm_stack_opm valid_arg11 Hvalid_arg2 Hvalid_sb' Hvalid_sb
+      eq_fcmp_arg11_arg2 stk mem strg ctx Hlen) as Hcmp_eval.
+    destruct Hcmp_eval as [vv [eval_arg11_vv eval_arg2_vv]].
     
     injection eq_idx as eq_idx.
-    unfold eval_sstack_val in eval_arg1_vv.
-    unfold eval_sstack_val in eval_arg21_vv.
-    rewrite <- eq_idx in eval_arg1_vv. rewrite <- eq_idx in eval_arg1.
+    unfold eval_sstack_val in eval_arg11_vv.
+    unfold eval_sstack_val in eval_arg2_vv.
+    rewrite <- eq_idx in eval_arg2_vv. rewrite <- eq_idx in eval_arg11.
     rewrite -> eval_arg1 in eval_arg1_vv.
     pose proof (not_basic_value_smv_symop AND [arg21;arg22]) as not_basic_and.
     apply Himpl in not_basic_and.
@@ -364,7 +417,7 @@ split.
       injection eval_arg22' as eq_arg22v_arg1v.
       rewrite -> eq_arg22v_arg1v.
       rewrite <- wand_wand1_2.
-      reflexivity.
+      reflexivity.*)
 Qed.
 
-End Opt_and_and1.
+End Opt_and_and2.
